Simplify NEWSTEP and fix proof accordingly...

backend/LinearC.v
@@ -3,10 +3,52 @@ Require Import ASTC Integers Values MemoryC Events GlobalenvsC Smallstep.
 Require Import Op LocationsC LTL Conventions.
 (** newly added **)
 Require Export Linear.
-Require Import ModSem.
-Require Import AsmregsC.
+Require Import Skeleton Mod ModSem.
+Require Import Simulation AsmregsC.
 
 Set Implicit Arguments.
+
+
+
+Section LINEAREXTRA.
+
+  Definition is_external (ge: genv) (st: state): Prop :=
+    match st with
+    | Callstate stack fptr sg ls m =>
+      match Genv.find_funct ge fptr with
+      | Some (AST.External ef) => is_external_ef ef
+      | _ => False
+      end
+    | _ => False
+    end
+  .
+
+  Variable ge: genv.
+  Definition semantics_with_ge := Semantics step bot1 final_state ge.
+  (* *************** ge is parameterized *******************)
+
+  Lemma semantics_receptive
+        st
+        (INTERNAL: ~is_external semantics_with_ge.(globalenv) st)
+    :
+      receptive_at semantics_with_ge st
+  .
+  Proof.
+    admit "this should hold".
+  Qed.
+
+  Lemma semantics_determinate
+        st
+        (INTERNAL: ~is_external semantics_with_ge.(globalenv) st)
+    :
+      determinate_at semantics_with_ge st
+  .
+  Proof.
+    admit "this should hold".
+  Qed.
+
+End LINEAREXTRA.
+(*** !!!!!!!!!!!!!!! REMOVE ABOVE AFTER MERGING WITH MIXED SIM BRANCH !!!!!!!!!!!!!!!!!! ***)
 
 
 
@@ -15,120 +57,136 @@ Section NEWSTEP.
 Variable ge: genv.
 Let find_function_ptr := find_function_ptr ge.
 
+Definition get_stack (st: state): list stackframe :=
+  match st with
+  | State stk _ _ _ _ _ => stk
+  | Callstate stk _ _ _ _ => stk
+  | Returnstate stk _ _ => stk
+  end.
+
 Inductive step: state -> trace -> state -> Prop :=
-  | exec_Lgetstack:
-      forall s f sp sl ofs ty dst b rs m rs',
-      rs' = Locmap.set (R dst) (rs (S sl ofs ty)) (LTL.undef_regs (destroyed_by_getstack sl) rs) ->
-      step (State s f sp (Lgetstack sl ofs ty dst :: b) rs m)
-        E0 (State s f sp b rs' m)
-  | exec_Lsetstack:
-      forall s f sp src sl ofs ty b rs m rs',
-      rs' = Locmap.set (S sl ofs ty) (rs (R src)) (LTL.undef_regs (destroyed_by_setstack ty) rs) ->
-      step (State s f sp (Lsetstack src sl ofs ty :: b) rs m)
-        E0 (State s f sp b rs' m)
-  | exec_Lop:
-      forall s f sp op args res b rs m v rs',
-      eval_operation ge sp op (reglist rs args) m = Some v ->
-      rs' = Locmap.set (R res) v (LTL.undef_regs (destroyed_by_op op) rs) ->
-      step (State s f sp (Lop op args res :: b) rs m)
-        E0 (State s f sp b rs' m)
-  | exec_Lload:
-      forall s f sp chunk addr args dst b rs m a v rs',
-      eval_addressing ge sp addr (reglist rs args) = Some a ->
-      Mem.loadv chunk m a = Some v ->
-      rs' = Locmap.set (R dst) v (LTL.undef_regs (destroyed_by_load chunk addr) rs) ->
-      step (State s f sp (Lload chunk addr args dst :: b) rs m)
-        E0 (State s f sp b rs' m)
-  | exec_Lstore:
-      forall s f sp chunk addr args src b rs m m' a rs',
-      eval_addressing ge sp addr (reglist rs args) = Some a ->
-      Mem.storev chunk m a (rs (R src)) = Some m' ->
-      rs' = LTL.undef_regs (destroyed_by_store chunk addr) rs ->
-      step (State s f sp (Lstore chunk addr args src :: b) rs m)
-        E0 (State s f sp b rs' m')
-  | exec_Lcall:
-      forall s f sp sig ros b rs m fptr
-      (FPTR: find_function_ptr ros rs m= fptr)
-      ,
-      DUMMY_PROP ->
-      DUMMY_PROP ->
-      step (State s f sp (Lcall sig ros :: b) rs m)
-        E0 (Callstate (Stackframe f sp rs b:: s) fptr sig rs m)
-  | exec_Ltailcall:
-      forall s f stk sig ros b rs m rs' fptr m'
-      (FPTR: find_function_ptr ros rs' m= fptr)
-      ,
-      rs' = return_regs (parent_locset s) rs ->
-      DUMMY_PROP ->
-      DUMMY_PROP ->
-      Mem.free m stk 0 f.(fn_stacksize) = Some m' ->
-      step (State s f (Vptr stk Ptrofs.zero true) (Ltailcall sig ros :: b) rs m)
-        E0 (Callstate s fptr sig rs' m')
-  | exec_Lbuiltin:
-      forall s f sp rs m ef args res b vargs t vres rs' m',
-      eval_builtin_args ge rs sp m args vargs ->
-      external_call ef ge vargs m t vres m' ->
-      rs' = Locmap.setres res vres (LTL.undef_regs (destroyed_by_builtin ef) rs) ->
-      step (State s f sp (Lbuiltin ef args res :: b) rs m)
-         t (State s f sp b rs' m')
-  | exec_Llabel:
-      forall s f sp lbl b rs m,
-      step (State s f sp (Llabel lbl :: b) rs m)
-        E0 (State s f sp b rs m)
-  | exec_Lgoto:
-      forall s f sp lbl b rs m b',
-      find_label lbl f.(fn_code) = Some b' ->
-      step (State s f sp (Lgoto lbl :: b) rs m)
-        E0 (State s f sp b' rs m)
-  | exec_Lcond_true:
-      forall s f sp cond args lbl b rs m rs' b',
-      eval_condition cond (reglist rs args) m = Some true ->
-      rs' = LTL.undef_regs (destroyed_by_cond cond) rs ->
-      find_label lbl f.(fn_code) = Some b' ->
-      step (State s f sp (Lcond cond args lbl :: b) rs m)
-        E0 (State s f sp b' rs' m)
-  | exec_Lcond_false:
-      forall s f sp cond args lbl b rs m rs',
-      eval_condition cond (reglist rs args) m = Some false ->
-      rs' = LTL.undef_regs (destroyed_by_cond cond) rs ->
-      step (State s f sp (Lcond cond args lbl :: b) rs m)
-        E0 (State s f sp b rs' m)
-  | exec_Ljumptable:
-      forall s f sp arg tbl b rs m n lbl b' rs',
-      rs (R arg) = Vint n ->
-      list_nth_z tbl (Int.unsigned n) = Some lbl ->
-      find_label lbl f.(fn_code) = Some b' ->
-      rs' = LTL.undef_regs (destroyed_by_jumptable) rs ->
-      step (State s f sp (Ljumptable arg tbl :: b) rs m)
-        E0 (State s f sp b' rs' m)
-  | exec_Lreturn:
-      forall s f stk b rs m m',
-      Mem.free m stk 0 f.(fn_stacksize) = Some m' ->
-      step (State s f (Vptr stk Ptrofs.zero true) (Lreturn :: b) rs m)
-        E0 (Returnstate s (return_regs (parent_locset s) rs) m')
-  | exec_function_internal:
-      forall s fptr sg f rs m rs' m' stk
-      (FPTR: Genv.find_funct ge fptr = Some (Internal f))
-      (SIG: sg = funsig (Internal f))
-      ,
-      Mem.alloc m 0 f.(fn_stacksize) = (m', stk) ->
-      rs' = LTL.undef_regs destroyed_at_function_entry (call_regs rs) ->
-      step (Callstate s fptr sg rs m)
-        E0 (State s f (Vptr stk Ptrofs.zero true) f.(fn_code) rs' m')
-  | exec_function_external:
-      forall s fptr sg ef args res rs1 rs2 m t m'
-      (FPTR: Genv.find_funct ge fptr = Some (External ef))
-      (SIG: sg = funsig (External ef))
-      ,
-      args = map (fun p => Locmap.getpair p rs1) (loc_arguments (ef_sig ef)) ->
-      external_call ef ge args m t res m' ->
-      rs2 = Locmap.setpair (loc_result (ef_sig ef)) res (LTL.undef_regs destroyed_at_call rs1) ->
-      step (Callstate s fptr sg rs1 m)
-         t (Returnstate s rs2 m')
-  | exec_return:
-      forall s f sp rs0 c rs m (NOTDUMMY: s <> []),
-      step (Returnstate (Stackframe f sp rs0 c :: s) rs m)
-        E0 (State s f sp c rs m).
+| step_intro
+    st0 tr st1
+    (STEP: Linear.step ge st0 tr st1)
+    (NOTDUMMY: st1.(get_stack) <> [])
+  :
+    step st0 tr st1
+.
+
+(* Inductive step: state -> trace -> state -> Prop := *)
+(*   | exec_Lgetstack: *)
+(*       forall s f sp sl ofs ty dst b rs m rs', *)
+(*       rs' = Locmap.set (R dst) (rs (S sl ofs ty)) (LTL.undef_regs (destroyed_by_getstack sl) rs) -> *)
+(*       step (State s f sp (Lgetstack sl ofs ty dst :: b) rs m) *)
+(*         E0 (State s f sp b rs' m) *)
+(*   | exec_Lsetstack: *)
+(*       forall s f sp src sl ofs ty b rs m rs', *)
+(*       rs' = Locmap.set (S sl ofs ty) (rs (R src)) (LTL.undef_regs (destroyed_by_setstack ty) rs) -> *)
+(*       step (State s f sp (Lsetstack src sl ofs ty :: b) rs m) *)
+(*         E0 (State s f sp b rs' m) *)
+(*   | exec_Lop: *)
+(*       forall s f sp op args res b rs m v rs', *)
+(*       eval_operation ge sp op (reglist rs args) m = Some v -> *)
+(*       rs' = Locmap.set (R res) v (LTL.undef_regs (destroyed_by_op op) rs) -> *)
+(*       step (State s f sp (Lop op args res :: b) rs m) *)
+(*         E0 (State s f sp b rs' m) *)
+(*   | exec_Lload: *)
+(*       forall s f sp chunk addr args dst b rs m a v rs', *)
+(*       eval_addressing ge sp addr (reglist rs args) = Some a -> *)
+(*       Mem.loadv chunk m a = Some v -> *)
+(*       rs' = Locmap.set (R dst) v (LTL.undef_regs (destroyed_by_load chunk addr) rs) -> *)
+(*       step (State s f sp (Lload chunk addr args dst :: b) rs m) *)
+(*         E0 (State s f sp b rs' m) *)
+(*   | exec_Lstore: *)
+(*       forall s f sp chunk addr args src b rs m m' a rs', *)
+(*       eval_addressing ge sp addr (reglist rs args) = Some a -> *)
+(*       Mem.storev chunk m a (rs (R src)) = Some m' -> *)
+(*       rs' = LTL.undef_regs (destroyed_by_store chunk addr) rs -> *)
+(*       step (State s f sp (Lstore chunk addr args src :: b) rs m) *)
+(*         E0 (State s f sp b rs' m') *)
+(*   | exec_Lcall: *)
+(*       forall s f sp sig ros b rs m fptr *)
+(*       (FPTR: find_function_ptr ros rs m= fptr) *)
+(*       , *)
+(*       DUMMY_PROP -> *)
+(*       DUMMY_PROP -> *)
+(*       step (State s f sp (Lcall sig ros :: b) rs m) *)
+(*         E0 (Callstate (Stackframe f sp rs b:: s) fptr sig rs m) *)
+(*   | exec_Ltailcall: *)
+(*       forall s f stk sig ros b rs m rs' fptr m' *)
+(*       (FPTR: find_function_ptr ros rs' m= fptr) *)
+(*       , *)
+(*       rs' = return_regs (parent_locset s) rs -> *)
+(*       DUMMY_PROP -> *)
+(*       DUMMY_PROP -> *)
+(*       Mem.free m stk 0 f.(fn_stacksize) = Some m' -> *)
+(*       step (State s f (Vptr stk Ptrofs.zero true) (Ltailcall sig ros :: b) rs m) *)
+(*         E0 (Callstate s fptr sig rs' m') *)
+(*   | exec_Lbuiltin: *)
+(*       forall s f sp rs m ef args res b vargs t vres rs' m', *)
+(*       eval_builtin_args ge rs sp m args vargs -> *)
+(*       external_call ef ge vargs m t vres m' -> *)
+(*       rs' = Locmap.setres res vres (LTL.undef_regs (destroyed_by_builtin ef) rs) -> *)
+(*       step (State s f sp (Lbuiltin ef args res :: b) rs m) *)
+(*          t (State s f sp b rs' m') *)
+(*   | exec_Llabel: *)
+(*       forall s f sp lbl b rs m, *)
+(*       step (State s f sp (Llabel lbl :: b) rs m) *)
+(*         E0 (State s f sp b rs m) *)
+(*   | exec_Lgoto: *)
+(*       forall s f sp lbl b rs m b', *)
+(*       find_label lbl f.(fn_code) = Some b' -> *)
+(*       step (State s f sp (Lgoto lbl :: b) rs m) *)
+(*         E0 (State s f sp b' rs m) *)
+(*   | exec_Lcond_true: *)
+(*       forall s f sp cond args lbl b rs m rs' b', *)
+(*       eval_condition cond (reglist rs args) m = Some true -> *)
+(*       rs' = LTL.undef_regs (destroyed_by_cond cond) rs -> *)
+(*       find_label lbl f.(fn_code) = Some b' -> *)
+(*       step (State s f sp (Lcond cond args lbl :: b) rs m) *)
+(*         E0 (State s f sp b' rs' m) *)
+(*   | exec_Lcond_false: *)
+(*       forall s f sp cond args lbl b rs m rs', *)
+(*       eval_condition cond (reglist rs args) m = Some false -> *)
+(*       rs' = LTL.undef_regs (destroyed_by_cond cond) rs -> *)
+(*       step (State s f sp (Lcond cond args lbl :: b) rs m) *)
+(*         E0 (State s f sp b rs' m) *)
+(*   | exec_Ljumptable: *)
+(*       forall s f sp arg tbl b rs m n lbl b' rs', *)
+(*       rs (R arg) = Vint n -> *)
+(*       list_nth_z tbl (Int.unsigned n) = Some lbl -> *)
+(*       find_label lbl f.(fn_code) = Some b' -> *)
+(*       rs' = LTL.undef_regs (destroyed_by_jumptable) rs -> *)
+(*       step (State s f sp (Ljumptable arg tbl :: b) rs m) *)
+(*         E0 (State s f sp b' rs' m) *)
+(*   | exec_Lreturn: *)
+(*       forall s f stk b rs m m', *)
+(*       Mem.free m stk 0 f.(fn_stacksize) = Some m' -> *)
+(*       step (State s f (Vptr stk Ptrofs.zero true) (Lreturn :: b) rs m) *)
+(*         E0 (Returnstate s (return_regs (parent_locset s) rs) m') *)
+(*   | exec_function_internal: *)
+(*       forall s fptr sg f rs m rs' m' stk *)
+(*       (FPTR: Genv.find_funct ge fptr = Some (Internal f)) *)
+(*       (SIG: sg = funsig (Internal f)) *)
+(*       , *)
+(*       Mem.alloc m 0 f.(fn_stacksize) = (m', stk) -> *)
+(*       rs' = LTL.undef_regs destroyed_at_function_entry (call_regs rs) -> *)
+(*       step (Callstate s fptr sg rs m) *)
+(*         E0 (State s f (Vptr stk Ptrofs.zero true) f.(fn_code) rs' m') *)
+(*   | exec_function_external: *)
+(*       forall s fptr sg ef args res rs1 rs2 m t m' *)
+(*       (FPTR: Genv.find_funct ge fptr = Some (External ef)) *)
+(*       (SIG: sg = funsig (External ef)) *)
+(*       , *)
+(*       args = map (fun p => Locmap.getpair p rs1) (loc_arguments (ef_sig ef)) -> *)
+(*       external_call ef ge args m t res m' -> *)
+(*       rs2 = Locmap.setpair (loc_result (ef_sig ef)) res (LTL.undef_regs destroyed_at_call rs1) -> *)
+(*       step (Callstate s fptr sg rs1 m) *)
+(*          t (Returnstate s rs2 m') *)
+(*   | exec_return: *)
+(*       forall s f sp rs0 c rs m (NOTDUMMY: s <> []), *)
+(*       step (Returnstate (Stackframe f sp rs0 c :: s) rs m) *)
+(*         E0 (State s f sp c rs m). *)
 
 End NEWSTEP.
 
@@ -198,8 +256,10 @@ Definition to_regset (ls: locset): regset :=
 
 Section MODSEM.
 
+  Variable skenv_link: SkEnv.t.
   Variable p: program.
-  Let ge := p.(Genv.globalenv).
+  Let skenv: SkEnv.t := skenv_link.(SkEnv.project) p.(defs).
+  Let ge: genv := skenv.(SkEnv.revive) p.
 
   Inductive at_external: state -> regset -> mem -> Prop :=
   | at_external_intro
@@ -280,7 +340,7 @@ Section MODSEM.
       ModSem.final_frame := final_frame;
       ModSem.after_external := after_external;
       ModSem.globalenv := ge; (* TODO: Change this properly *)
-      ModSem.skenv := (admit "TODO")
+      ModSem.skenv := skenv;
     |}
   .
   Next Obligation. all_prop_inv; ss. Qed.
@@ -294,7 +354,7 @@ Section MODSEM.
   Next Obligation. all_prop_inv; ss. Qed.
   Next Obligation. all_prop_inv; ss. Qed.
   Next Obligation.
-    ii. des. inv PR. inv PR0; ss; clarify.
+    ii. des. inv PR. inv PR0; inv STEP; ss; clarify.
     (* hnf. inv H4; inv H2; subst_locals; all_rewrite; ss; des_ifs. *)
   Qed.
   Next Obligation. ii. des. all_prop_inv; ss. Qed.
