backend/MachC.v
@@ -13,10 +13,62 @@ Require Import Conventions.
 Require Stacklayout.
 (** newly added **)
 Require Export Mach.
-Require Import ModSem.
-Require Import Integers.
+Require Import Skeleton Mod ModSem.
+Require Import Simulation Integers.
 
 Set Implicit Arguments.
+
+
+
+Section MACHEXTRA.
+
+  Variable rao: function -> code -> ptrofs -> Prop.
+
+  Hypothesis rao_dtm:
+    forall f c ofs ofs',
+      rao f c ofs ->
+      rao f c ofs' ->
+      ofs = ofs'. 
+
+  Definition is_external (ge: genv) (st: state): Prop :=
+    match st with
+    | Callstate stack fptr rs m =>
+      match Genv.find_funct ge fptr with
+      | Some (AST.External ef) => is_external_ef ef
+      | _ => False
+      end
+    | _ => False
+    end
+  .
+
+  Variable ge: genv.
+  Definition semantics_with_ge := Semantics (step rao) bot1 final_state ge.
+  (* *************** ge is parameterized *******************)
+
+  Lemma semantics_receptive
+        st
+        (INTERNAL: ~is_external semantics_with_ge.(globalenv) st)
+    :
+      receptive_at semantics_with_ge st
+  .
+  Proof.
+    revert rao_dtm. (* dummy *)
+    admit "this should hold".
+  Qed.
+
+  Lemma semantics_determinate
+        st
+        (INTERNAL: ~is_external semantics_with_ge.(globalenv) st)
+    :
+      determinate_at semantics_with_ge st
+  .
+  Proof.
+    revert rao_dtm. (* dummy *)
+    admit "this should hold".
+  Qed.
+
+End MACHEXTRA.
+(*** !!!!!!!!!!!!!!! REMOVE ABOVE AFTER MERGING WITH MIXED SIM BRANCH !!!!!!!!!!!!!!!!!! ***)
 
 
 
@@ -25,134 +77,150 @@ Section NEWSTEP.
 Variable return_address_offset: function -> code -> ptrofs -> Prop.
 Variable ge: genv.
 
+Definition get_stack (st: state): list stackframe :=
+  match st with
+  | State stk _ _ _ _ _ => stk
+  | Callstate stk _ _ _ => stk
+  | Returnstate stk _ _ => stk
+  end.
+
 Inductive step: state -> trace -> state -> Prop :=
-  | exec_Mlabel:
-      forall s f sp lbl c rs m,
-      step (State s f sp (Mlabel lbl :: c) rs m)
-        E0 (State s f sp c rs m)
-  | exec_Mgetstack:
-      forall s f sp ofs ty dst c rs m v,
-      load_stack m sp ty ofs = Some v ->
-      step (State s f sp (Mgetstack ofs ty dst :: c) rs m)
-        E0 (State s f sp c (rs#dst <- v) m)
-  | exec_Msetstack:
-      forall s f sp src ofs ty c rs m m' rs',
-      store_stack m sp ty ofs (rs src) = Some m' ->
-      rs' = undef_regs (destroyed_by_setstack ty) rs ->
-      step (State s f sp (Msetstack src ofs ty :: c) rs m)
-        E0 (State s f sp c rs' m')
-  | exec_Mgetparam:
-      forall s fb f sp ofs ty dst c rs m v rs',
-      Genv.find_funct_ptr ge fb = Some (Internal f) ->
-      load_stack m sp Tptr f.(fn_link_ofs) = Some (parent_sp s) ->
-      load_stack m (parent_sp s) ty ofs = Some v ->
-      rs' = (rs # temp_for_parent_frame <- Vundef # dst <- v) ->
-      step (State s fb sp (Mgetparam ofs ty dst :: c) rs m)
-        E0 (State s fb sp c rs' m)
-  | exec_Mop:
-      forall s f sp op args res c rs m v rs',
-      eval_operation ge sp op rs##args m = Some v ->
-      rs' = ((undef_regs (destroyed_by_op op) rs)#res <- v) ->
-      step (State s f sp (Mop op args res :: c) rs m)
-        E0 (State s f sp c rs' m)
-  | exec_Mload:
-      forall s f sp chunk addr args dst c rs m a v rs',
-      eval_addressing ge sp addr rs##args = Some a ->
-      Mem.loadv chunk m a = Some v ->
-      rs' = ((undef_regs (destroyed_by_load chunk addr) rs)#dst <- v) ->
-      step (State s f sp (Mload chunk addr args dst :: c) rs m)
-        E0 (State s f sp c rs' m)
-  | exec_Mstore:
-      forall s f sp chunk addr args src c rs m m' a rs',
-      eval_addressing ge sp addr rs##args = Some a ->
-      Mem.storev chunk m a (rs src) = Some m' ->
-      rs' = undef_regs (destroyed_by_store chunk addr) rs ->
-      step (State s f sp (Mstore chunk addr args src :: c) rs m)
-        E0 (State s f sp c rs' m')
-  | exec_Mcall:
-      forall s fb sp sig ros c rs m f f' ra,
-      find_function_ptr ge ros rs m= f' ->
-      Genv.find_funct_ptr ge fb = Some (Internal f) ->
-      return_address_offset f c ra ->
-      step (State s fb sp (Mcall sig ros :: c) rs m)
-        E0 (Callstate (Stackframe fb sp (Vptr fb ra true) c :: s)
-                       f' rs m)
-  | exec_Mtailcall:
-      forall s fb stk soff sig ros c rs m f f' m',
-      find_function_ptr ge ros rs m= f' ->
-      Genv.find_funct_ptr ge fb = Some (Internal f) ->
-      load_stack m (Vptr stk soff true) Tptr f.(fn_link_ofs) = Some (parent_sp s) ->
-      load_stack m (Vptr stk soff true) Tptr f.(fn_retaddr_ofs) = Some (parent_ra s) ->
-      Mem.free m stk 0 f.(fn_stacksize) = Some m' ->
-      step (State s fb (Vptr stk soff true) (Mtailcall sig ros :: c) rs m)
-        E0 (Callstate s f' rs m')
-  | exec_Mbuiltin:
-      forall s f sp rs m ef args res b vargs t vres rs' m',
-      eval_builtin_args ge rs sp m args vargs ->
-      external_call ef ge vargs m t vres m' ->
-      rs' = set_res res vres (undef_regs (destroyed_by_builtin ef) rs) ->
-      step (State s f sp (Mbuiltin ef args res :: b) rs m)
-         t (State s f sp b rs' m')
-  | exec_Mgoto:
-      forall s fb f sp lbl c rs m c',
-      Genv.find_funct_ptr ge fb = Some (Internal f) ->
-      find_label lbl f.(fn_code) = Some c' ->
-      step (State s fb sp (Mgoto lbl :: c) rs m)
-        E0 (State s fb sp c' rs m)
-  | exec_Mcond_true:
-      forall s fb f sp cond args lbl c rs m c' rs',
-      eval_condition cond rs##args m = Some true ->
-      Genv.find_funct_ptr ge fb = Some (Internal f) ->
-      find_label lbl f.(fn_code) = Some c' ->
-      rs' = undef_regs (destroyed_by_cond cond) rs ->
-      step (State s fb sp (Mcond cond args lbl :: c) rs m)
-        E0 (State s fb sp c' rs' m)
-  | exec_Mcond_false:
-      forall s f sp cond args lbl c rs m rs',
-      eval_condition cond rs##args m = Some false ->
-      rs' = undef_regs (destroyed_by_cond cond) rs ->
-      step (State s f sp (Mcond cond args lbl :: c) rs m)
-        E0 (State s f sp c rs' m)
-  | exec_Mjumptable:
-      forall s fb f sp arg tbl c rs m n lbl c' rs',
-      rs arg = Vint n ->
-      list_nth_z tbl (Int.unsigned n) = Some lbl ->
-      Genv.find_funct_ptr ge fb = Some (Internal f) ->
-      find_label lbl f.(fn_code) = Some c' ->
-      rs' = undef_regs destroyed_by_jumptable rs ->
-      step (State s fb sp (Mjumptable arg tbl :: c) rs m)
-        E0 (State s fb sp c' rs' m)
-  | exec_Mreturn:
-      forall s fb stk soff c rs m f m',
-      Genv.find_funct_ptr ge fb = Some (Internal f) ->
-      load_stack m (Vptr stk soff true) Tptr f.(fn_link_ofs) = Some (parent_sp s) ->
-      load_stack m (Vptr stk soff true) Tptr f.(fn_retaddr_ofs) = Some (parent_ra s) ->
-      Mem.free m stk 0 f.(fn_stacksize) = Some m' ->
-      step (State s fb (Vptr stk soff true) (Mreturn :: c) rs m)
-        E0 (Returnstate s rs m')
-  | exec_function_internal:
-      forall s fptr fb rs m f m1 m2 m3 stk rs'
-      (FPTR: fptr = Vptr fb Ptrofs.zero true),
-      Genv.find_funct_ptr ge fb = Some (Internal f) ->
-      Mem.alloc m 0 f.(fn_stacksize) = (m1, stk) ->
-      let sp := Vptr stk Ptrofs.zero true in
-      store_stack m1 sp Tptr f.(fn_link_ofs) (parent_sp s) = Some m2 ->
-      store_stack m2 sp Tptr f.(fn_retaddr_ofs) (parent_ra s) = Some m3 ->
-      rs' = undef_regs destroyed_at_function_entry rs ->
-      step (Callstate s fptr rs m)
-        E0 (State s fb sp f.(fn_code) rs' m3)
-  | exec_function_external:
-      forall s fb rs m t rs' ef args res m',
-      Genv.find_funct ge fb = Some (External ef) ->
-      extcall_arguments rs m (parent_sp s) (ef_sig ef) args ->
-      external_call ef ge args m t res m' ->
-      rs' = set_pair (loc_result (ef_sig ef)) res (undef_regs destroyed_at_call rs) ->
-      step (Callstate s fb rs m)
-         t (Returnstate s rs' m')
-  | exec_return:
-      forall s f sp ra c rs m (NOTDUMMY: s <> []),
-      step (Returnstate (Stackframe f sp ra c :: s) rs m)
-        E0 (State s f sp c rs m).
+| step_intro
+    st0 tr st1
+    (STEP: Mach.step return_address_offset ge st0 tr st1)
+    (NOTDUMMY: st1.(get_stack) <> [])
+  :
+    step st0 tr st1
+.
+
+(* Inductive step: state -> trace -> state -> Prop := *)
+(*   | exec_Mlabel: *)
+(*       forall s f sp lbl c rs m, *)
+(*       step (State s f sp (Mlabel lbl :: c) rs m) *)
+(*         E0 (State s f sp c rs m) *)
+(*   | exec_Mgetstack: *)
+(*       forall s f sp ofs ty dst c rs m v, *)
+(*       load_stack m sp ty ofs = Some v -> *)
+(*       step (State s f sp (Mgetstack ofs ty dst :: c) rs m) *)
+(*         E0 (State s f sp c (rs#dst <- v) m) *)
+(*   | exec_Msetstack: *)
+(*       forall s f sp src ofs ty c rs m m' rs', *)
+(*       store_stack m sp ty ofs (rs src) = Some m' -> *)
+(*       rs' = undef_regs (destroyed_by_setstack ty) rs -> *)
+(*       step (State s f sp (Msetstack src ofs ty :: c) rs m) *)
+(*         E0 (State s f sp c rs' m') *)
+(*   | exec_Mgetparam: *)
+(*       forall s fb f sp ofs ty dst c rs m v rs', *)
+(*       Genv.find_funct_ptr ge fb = Some (Internal f) -> *)
+(*       load_stack m sp Tptr f.(fn_link_ofs) = Some (parent_sp s) -> *)
+(*       load_stack m (parent_sp s) ty ofs = Some v -> *)
+(*       rs' = (rs # temp_for_parent_frame <- Vundef # dst <- v) -> *)
+(*       step (State s fb sp (Mgetparam ofs ty dst :: c) rs m) *)
+(*         E0 (State s fb sp c rs' m) *)
+(*   | exec_Mop: *)
+(*       forall s f sp op args res c rs m v rs', *)
+(*       eval_operation ge sp op rs##args m = Some v -> *)
+(*       rs' = ((undef_regs (destroyed_by_op op) rs)#res <- v) -> *)
+(*       step (State s f sp (Mop op args res :: c) rs m) *)
+(*         E0 (State s f sp c rs' m) *)
+(*   | exec_Mload: *)
+(*       forall s f sp chunk addr args dst c rs m a v rs', *)
+(*       eval_addressing ge sp addr rs##args = Some a -> *)
+(*       Mem.loadv chunk m a = Some v -> *)
+(*       rs' = ((undef_regs (destroyed_by_load chunk addr) rs)#dst <- v) -> *)
+(*       step (State s f sp (Mload chunk addr args dst :: c) rs m) *)
+(*         E0 (State s f sp c rs' m) *)
+(*   | exec_Mstore: *)
+(*       forall s f sp chunk addr args src c rs m m' a rs', *)
+(*       eval_addressing ge sp addr rs##args = Some a -> *)
+(*       Mem.storev chunk m a (rs src) = Some m' -> *)
+(*       rs' = undef_regs (destroyed_by_store chunk addr) rs -> *)
+(*       step (State s f sp (Mstore chunk addr args src :: c) rs m) *)
+(*         E0 (State s f sp c rs' m') *)
+(*   | exec_Mcall: *)
+(*       forall s fb sp sig ros c rs m f f' ra, *)
+(*       find_function_ptr ge ros rs m= f' -> *)
+(*       Genv.find_funct_ptr ge fb = Some (Internal f) -> *)
+(*       return_address_offset f c ra -> *)
+(*       step (State s fb sp (Mcall sig ros :: c) rs m) *)
+(*         E0 (Callstate (Stackframe fb sp (Vptr fb ra true) c :: s) *)
+(*                        f' rs m) *)
+(*   | exec_Mtailcall: *)
+(*       forall s fb stk soff sig ros c rs m f f' m', *)
+(*       find_function_ptr ge ros rs m= f' -> *)
+(*       Genv.find_funct_ptr ge fb = Some (Internal f) -> *)
+(*       load_stack m (Vptr stk soff true) Tptr f.(fn_link_ofs) = Some (parent_sp s) -> *)
+(*       load_stack m (Vptr stk soff true) Tptr f.(fn_retaddr_ofs) = Some (parent_ra s) -> *)
+(*       Mem.free m stk 0 f.(fn_stacksize) = Some m' -> *)
+(*       step (State s fb (Vptr stk soff true) (Mtailcall sig ros :: c) rs m) *)
+(*         E0 (Callstate s f' rs m') *)
+(*   | exec_Mbuiltin: *)
+(*       forall s f sp rs m ef args res b vargs t vres rs' m', *)
+(*       eval_builtin_args ge rs sp m args vargs -> *)
+(*       external_call ef ge vargs m t vres m' -> *)
+(*       rs' = set_res res vres (undef_regs (destroyed_by_builtin ef) rs) -> *)
+(*       step (State s f sp (Mbuiltin ef args res :: b) rs m) *)
+(*          t (State s f sp b rs' m') *)
+(*   | exec_Mgoto: *)
+(*       forall s fb f sp lbl c rs m c', *)
+(*       Genv.find_funct_ptr ge fb = Some (Internal f) -> *)
+(*       find_label lbl f.(fn_code) = Some c' -> *)
+(*       step (State s fb sp (Mgoto lbl :: c) rs m) *)
+(*         E0 (State s fb sp c' rs m) *)
+(*   | exec_Mcond_true: *)
+(*       forall s fb f sp cond args lbl c rs m c' rs', *)
+(*       eval_condition cond rs##args m = Some true -> *)
+(*       Genv.find_funct_ptr ge fb = Some (Internal f) -> *)
+(*       find_label lbl f.(fn_code) = Some c' -> *)
+(*       rs' = undef_regs (destroyed_by_cond cond) rs -> *)
+(*       step (State s fb sp (Mcond cond args lbl :: c) rs m) *)
+(*         E0 (State s fb sp c' rs' m) *)
+(*   | exec_Mcond_false: *)
+(*       forall s f sp cond args lbl c rs m rs', *)
+(*       eval_condition cond rs##args m = Some false -> *)
+(*       rs' = undef_regs (destroyed_by_cond cond) rs -> *)
+(*       step (State s f sp (Mcond cond args lbl :: c) rs m) *)
+(*         E0 (State s f sp c rs' m) *)
+(*   | exec_Mjumptable: *)
+(*       forall s fb f sp arg tbl c rs m n lbl c' rs', *)
+(*       rs arg = Vint n -> *)
+(*       list_nth_z tbl (Int.unsigned n) = Some lbl -> *)
+(*       Genv.find_funct_ptr ge fb = Some (Internal f) -> *)
+(*       find_label lbl f.(fn_code) = Some c' -> *)
+(*       rs' = undef_regs destroyed_by_jumptable rs -> *)
+(*       step (State s fb sp (Mjumptable arg tbl :: c) rs m) *)
+(*         E0 (State s fb sp c' rs' m) *)
+(*   | exec_Mreturn: *)
+(*       forall s fb stk soff c rs m f m', *)
+(*       Genv.find_funct_ptr ge fb = Some (Internal f) -> *)
+(*       load_stack m (Vptr stk soff true) Tptr f.(fn_link_ofs) = Some (parent_sp s) -> *)
+(*       load_stack m (Vptr stk soff true) Tptr f.(fn_retaddr_ofs) = Some (parent_ra s) -> *)
+(*       Mem.free m stk 0 f.(fn_stacksize) = Some m' -> *)
+(*       step (State s fb (Vptr stk soff true) (Mreturn :: c) rs m) *)
+(*         E0 (Returnstate s rs m') *)
+(*   | exec_function_internal: *)
+(*       forall s fptr fb rs m f m1 m2 m3 stk rs' *)
+(*       (FPTR: fptr = Vptr fb Ptrofs.zero true), *)
+(*       Genv.find_funct_ptr ge fb = Some (Internal f) -> *)
+(*       Mem.alloc m 0 f.(fn_stacksize) = (m1, stk) -> *)
+(*       let sp := Vptr stk Ptrofs.zero true in *)
+(*       store_stack m1 sp Tptr f.(fn_link_ofs) (parent_sp s) = Some m2 -> *)
+(*       store_stack m2 sp Tptr f.(fn_retaddr_ofs) (parent_ra s) = Some m3 -> *)
+(*       rs' = undef_regs destroyed_at_function_entry rs -> *)
+(*       step (Callstate s fptr rs m) *)
+(*         E0 (State s fb sp f.(fn_code) rs' m3) *)
+(*   | exec_function_external: *)
+(*       forall s fb rs m t rs' ef args res m', *)
+(*       Genv.find_funct ge fb = Some (External ef) -> *)
+(*       extcall_arguments rs m (parent_sp s) (ef_sig ef) args -> *)
+(*       external_call ef ge args m t res m' -> *)
+(*       rs' = set_pair (loc_result (ef_sig ef)) res (undef_regs destroyed_at_call rs) -> *)
+(*       step (Callstate s fb rs m) *)
+(*          t (Returnstate s rs' m') *)
+(*   | exec_return: *)
+(*       forall s f sp ra c rs m (NOTDUMMY: s <> []), *)
+(*       step (Returnstate (Stackframe f sp ra c :: s) rs m) *)
+(*         E0 (State s f sp c rs m). *)
 
 End NEWSTEP.
 
@@ -197,8 +265,17 @@ Coercion mregset_of: regset >-> Mach.regset.
 Section MODSEM.
 
   Variable rao: function -> code -> ptrofs -> Prop.
+  Hypothesis rao_dtm:
+    forall f c ofs ofs',
+      rao f c ofs ->
+      rao f c ofs' ->
+      ofs = ofs'. 
+
+
+  Variable skenv_link: SkEnv.t.
   Variable p: program.
-  Let ge := p.(Genv.globalenv).
+  Let skenv: SkEnv.t := skenv_link.(SkEnv.project) p.(defs).
+  Let ge: genv := skenv.(SkEnv.revive) p.
 
   Inductive at_external: state -> regset -> mem -> Prop :=
   | at_external_intro
@@ -256,8 +333,8 @@ Section MODSEM.
       ModSem.initial_frame := initial_frame;
       ModSem.final_frame := final_frame;
       ModSem.after_external := after_external;
-      ModSem.globalenv := ge; (* TODO: Change this properly *)
-      ModSem.skenv := (admit "TODO")
+      ModSem.globalenv := ge; 
+      ModSem.skenv := skenv;
     |}
   .
   Next Obligation. all_prop_inv; ss. Qed.
@@ -265,10 +342,71 @@ Section MODSEM.
   Next Obligation. all_prop_inv; ss. Qed.
   Next Obligation. all_prop_inv; ss. Qed.
   Next Obligation.
-    ii. des. inv PR. inv PR0; ss; all_rewrite; ss; des_ifs.
+    ii. des. inv PR. inv PR0; inv STEP; ss; all_rewrite; ss; des_ifs.
   Qed.
   Next Obligation. ii. des. all_prop_inv; ss. Qed.
   Next Obligation. ii. des. all_prop_inv; ss. Qed.
+
+  Lemma not_external
+    :
+      is_external ge <1= bot1
+  .
+  Proof.
+    ii. hnf in PR. des_ifs.
+    subst_locals.
+    unfold Genv.find_funct, Genv.find_funct_ptr in *. des_ifs.
+    repeat all_once_fast ltac:(fun H => try apply Genv_map_defs_spec in H; des).
+    Local Opaque Genv.invert_symbol.
+    unfold o_bind, o_join, o_map in *. cbn in *. des_ifs_safe.
+    unfold ASTC.is_external, is_external_fd in *. simpl_bool. des_ifs.
+  Qed.
+
+  Lemma lift_receptive_at
+        st
+        (RECEP: receptive_at (semantics_with_ge rao ge) st)
+    :
+      receptive_at modsem st
+  .
+  Proof.
+    inv RECEP. econs; eauto; ii; ss.
+    - inv H.
+      exploit sr_receptive_at; eauto.
+      { eapply match_traces_preserved; try eassumption. ii; ss. }
+      i; des. esplits; eauto. econs; eauto.
+      { admit "1) prove get_stack dtm 2) at first place, prove full determinacy instead of determinate". }
+    - inv H.
+      exploit sr_traces_at; eauto.
+  Qed.
+
+  Lemma modsem_receptive
+        st
+    :
+      receptive_at modsem st
+  .
+  Proof. eapply lift_receptive_at. eapply semantics_receptive; eauto. ii. eapply not_external; eauto. Qed.
+
+  Lemma lift_determinate_at
+        st0
+        (DTM: determinate_at (semantics_with_ge rao ge) st0)
+    :
+      determinate_at modsem st0
+  .
+  Proof.
+    inv DTM. econs; eauto; ii; ss.
+    - inv H. inv H0.
+      determ_tac sd_determ_at. esplits; eauto.
+      eapply match_traces_preserved; try eassumption. ii; ss.
+    - inv H.
+      exploit sd_traces_at; eauto.
+  Qed.
+
+  Lemma modsem_determinate
+        st
+    :
+      determinate_at modsem st
+  .
+  Proof. eapply lift_determinate_at. eapply semantics_determinate; eauto. ii. eapply not_external; eauto. Qed.
+
 
 End MODSEM.
 
